Term/WithArity/AMonAlg.v
@@ -15,11 +15,14 @@ References:
 
 Require Import AWFMInterpretation.
 
-Module Type WeaklyMonotoneAlgebra.
+(***********************************************************************)
+(** * Module type specifying a weakly monotone algebra.                *)
+(***********************************************************************)
+Module Type MonotoneAlgebraType.
 
   Parameter Sig: Signature.
     
-  (* 
+  (**
      A weakly monotone algebra consist of:
      - interpretation [I]
      - [gt] and [ge] relations
@@ -40,21 +43,28 @@ Module Type WeaklyMonotoneAlgebra.
 
   Parameter gt_ge_compat: absorb gt ge.
 
-End WeaklyMonotoneAlgebra.
+End MonotoneAlgebraType.
 
-Module Type ExtendedMonotoneAlgebra.
+(***********************************************************************)
+(** * Module type specifying an extended weakly monotone algebra.      *)
+(***********************************************************************)
+Module Type ExtendedMonotoneAlgebraType.
 
-  Declare Module WMA: WeaklyMonotoneAlgebra.
-  Export WMA.
+  Declare Module MA: MonotoneAlgebraType.
+  Export MA.
 
-  (* Extended monotone algebra needs to have strictly montone interpretations *)
+  (** Extended monotone algebra is a wekaly monotone algebra in which every operation
+      is monotone with respect to [gt] *)
   Parameter monotone_gt: monotone I gt.
 
-End ExtendedMonotoneAlgebra.
+End ExtendedMonotoneAlgebraType.
 
-Module MonotoneAlgebraResults (WMA : WeaklyMonotoneAlgebra).
+(***********************************************************************)
+(** * Functor with a theory of weakly monotone algebras                *)
+(***********************************************************************)
+Module MonotoneAlgebraResults (MA : MonotoneAlgebraType).
 
-  Export WMA.
+  Export MA.
   Require Import ACompat.
 
   Definition IR_gt := IR I gt.
@@ -89,7 +99,9 @@ Module MonotoneAlgebraResults (WMA : WeaklyMonotoneAlgebra).
     exact monotone_ge.
   Qed.
 
-  Section Termination.
+(**********************************************************************)
+(** top termination (for DP setting) criterion with monotone algebras *)
+  Section TopTermination.
 
     Variable R E : rules.
 
@@ -107,13 +119,45 @@ Module MonotoneAlgebraResults (WMA : WeaklyMonotoneAlgebra).
       unfold IR_gt. apply IR_WF. exact gt_wf.
     Qed.
 
-  End Termination.
+  End TopTermination.
+
+(**********************************************************)
+(** criterion for modular removal of rules for relative top
+    termination with monotone algebras *)
+  Section ModularTopTermination.
+
+    Variable R R' E : rules.
+
+    (* Modular removal of rules *)
+    Lemma ma_modular_hd_red_mod :
+      WF (hd_red_mod E R') ->
+      compatible IR_gt R ->
+      compatible IR_ge (R' ++ E) ->
+      WF (hd_red_mod E (R ++ R')).
+
+    Proof.
+      intros. unfold hd_red_mod.
+      apply WF_incl with (red E# @ (hd_red R' U hd_red R)).
+      comp. trans (hd_red (R' ++ R)). 
+      apply hd_red_swap. apply hd_red_union.
+      apply wf_rel_mod_simpl. assumption.
+      apply WF_incl with (hd_red_mod (R' ++ E) R).
+      unfold hd_red_mod. comp. apply incl_rtc. 
+      trans (red R' U red E). apply incl_union. apply hd_red_incl_red. intuition.
+      apply red_union_inv.
+      apply ma_compat_hd_red_mod; trivial.
+    Qed.
+
+  End ModularTopTermination.
 
 End MonotoneAlgebraResults.
 
-Module ExtendedMonotoneAlgebraResults (EMA: ExtendedMonotoneAlgebra).
+(***********************************************************************)
+(** * Functor with a theory of extended monotone algebras              *)
+(***********************************************************************)
+Module ExtendedMonotoneAlgebraResults (EMA: ExtendedMonotoneAlgebraType).
 
-  Module MAR := MonotoneAlgebraResults EMA.WMA.
+  Module MAR := MonotoneAlgebraResults EMA.MA.
   Export MAR.
   Export EMA.
 
@@ -126,10 +170,13 @@ Module ExtendedMonotoneAlgebraResults (EMA: ExtendedMonotoneAlgebra).
     exact monotone_gt.
   Qed.
 
-  Section Termination.
+(**********************************************************)
+(** relative termination criterion with monotone algebras *)
+  Section RelativeTermination.
 
     Variable R E : rules.
 
+    (* Termination in one go *)
     Lemma ma_compat_red_mod : 
       compatible IR_gt R ->
       compatible IR_ge E ->
@@ -144,6 +191,35 @@ Module ExtendedMonotoneAlgebraResults (EMA: ExtendedMonotoneAlgebra).
       unfold IR_gt. apply IR_WF. exact gt_wf.
     Qed.
 
-  End Termination.
+  End RelativeTermination.
+
+(**********************************************************)
+(** criterion for modular removal of rules for relative 
+    termination with monotone algebras *)
+  Section ModularRelativeTermination.
+
+    Variable R E R' E' : rules.
+
+    (* Modular removal of rules *)
+    Lemma ma_modular_red_mod :
+      WF (red_mod E' R') ->
+      compatible IR_gt (R  ++ E ) ->
+      compatible IR_ge (R' ++ E') ->
+      WF (red_mod (E ++ E') (R ++ R')).
+
+    Proof.
+      intros. unfold red_mod.
+      apply WF_incl with ((red E' U red E)# @ (red R' U red R)).
+      comp. apply incl_rtc. 
+      trans (red (E' ++ E)). apply red_swap. apply red_union. 
+      trans (red (R' ++ R)). apply red_swap. apply red_union.
+      apply wf_rel_mod. fold (red_mod E' R'). assumption.
+      apply WF_incl with (red_mod (R' ++ E') (R ++ E)).
+      unfold red_mod. comp. 
+      apply incl_rtc. apply red_union_inv. apply red_union_inv.
+      apply ma_compat_red_mod; trivial.
+    Qed.
+
+  End ModularRelativeTermination.
 
 End ExtendedMonotoneAlgebraResults.
